%! Author = Len Washington III
%! Date = 9/16/24

% Preamble
\documentclass[
	date={September 16{,} 2024}
]{math486notes}

% Document
\begin{document}

Multiple Dosing. Two injections. Injection at $t=0$ and $t=t_{1}$.

\begin{equation*}
\begin{aligned}
	D\delta(t) + D\delta(t - t_{1})&\\
	\frac{dx}{dt} &= -kx + D\delta(t) + D\delta(t - t_{1}),\ \ x(0) = 0
\end{aligned}
\end{equation*}
\begin{equation*}
\begin{aligned}
	\laplace[\frac{dx}{dt}] &= \laplace[-kx] + \laplace[D\delta(t)] + \laplace[D\delta(t - t_{1})]\\
	sX(s) &= -k\laplace[x] + D\laplace[\delta(t)] + D\laplace[\delta(t - t_{1})]\\
	sX(s) &= -kX(s) + D(1) + De^{st_{1}}\\
	sX(s) + kX(s) &= D + De^{st_{1}}\\
	(s+k)X(s) &= D + De^{st_{1}}\\
	X(s) &= \frac{D}{s+k} + D\frac{e^{st_{1}}}{s+k}\\
	\laplacei[X(s)] &= \laplacei[\frac{D}{s+k}] + \laplacei[D\frac{e^{st_{1}}}{s+k}]\\
	x(t) &= D\laplacei[\frac{1}{s+k}] + D\laplacei[\frac{e^{st_{1}}}{s+k}]\\
	x(t) &= De^{-kt} + De^{-kt}\unitstep(t+t_{1})\\
		 &= De^{-kt} \left(1 + \unitstep(t+t_{1}) \right)\\
		 &= \left\{ \begin{array}{ll}
		 	De^{-kt} & 0 \leq t < t_{1}\\
			De^{-kt} + De^{-k(t-t_{1})} & t \geq t_{1}
		 \end{array} \right.
\end{aligned}
\end{equation*}

\section{Intermittent Infusion (IV)}\label{sec:intermittent-infusion}
Over finite time intended

\[ I(t) = \left\{ \begin{array}{cl}
	D & 0 \leq t < 1\\
	0 & t > 1
\end{array} \right. \]
\begin{equation*}
\begin{aligned}
	\frac{dx}{dt} = -kx + I(t),\ \ x(0) = 0,\ \ c = \frac{x}{volume}
\end{aligned}
\end{equation*}

How to model $I(t)$?
Want a one line formula to use Laplace Transform Table

\begin{equation}
	I(t) = D[ \unitstep(t) - \unitstep(t-1) ]
	\label{eq:}
\end{equation}

\begin{equation*}
\begin{aligned}
	\laplace[ \frac{dx}{dt} ] &= -kX(s) + D\left[ \laplace[\unitstep(t)] - \laplace[\unitstep(t-1)] \right]\\
	sX(s) - x(0) &= -kX(s) + D\left[ \frac{1}{s} - \frac{e^{-s}}{s} \right]\\
	sX(s) - 0 + kX(s) &= \frac{D}{s} - D\frac{e^{-s}}{s}\\
	(s+k)X(s) &= \frac{D}{s} - D\frac{e^{-s}}{s}\\
	X(s) &= \frac{D}{s(s+k)} - D\frac{e^{-s}}{s(s+k)}\\
\end{aligned}
\end{equation*}
\begin{equation*}
\begin{aligned}
	\frac{D}{s(s+k)} &= \frac{A}{s} + \frac{B}{s+k}\\
	\frac{D}{s(s+k)} &= \frac{A(s+k)}{s(s+k)} + \frac{Bs}{s(s+k)}\\
	D &= A(s+k) + Bs\\
\end{aligned}
\end{equation*}
Must be true for any $s$

\begin{minipage}[t]{0.5\textwidth}
	\begin{equation*}
	\begin{aligned}
		s &= 0\\
		D &= A(0+k) + B(0)\\
		D &= Ak\\
		A &= \frac{D}{k}\\
	\end{aligned}
	\end{equation*}
\end{minipage}%
\begin{minipage}[t]{0.5\textwidth}
	\begin{equation*}
	\begin{aligned}
		s &= -k\\
		D &= A(-k+k) + B(-k)\\
		D &= A(0) - Bk\\
		D &= -Bk\\
		B &= -\frac{D}{k}\\
	\end{aligned}
	\end{equation*}
\end{minipage}
\begin{equation*}
\begin{aligned}
	\frac{D}{s(s+k)} &= \frac{A}{s} + \frac{B}{s+k}\\
	\frac{D}{s(s+k)} &= \frac{D}{ks} - \frac{Dk^{-1}}{s+k}\\
\end{aligned}
\end{equation*}
\begin{equation*}
\begin{aligned}
	X(s) &= \frac{D}{s(s+k)} - D\frac{e^{-s}}{s(s+k)}\\
	X(s) &= \frac{Dk^{-1}}{s} - \frac{Dk^{-1}}{s+k} - De^{-s}\left[ \frac{Dk^{-1}}{s} - \frac{Dk^{-1}}{s+k} \right]\\
	\laplacei[X(s)] &= \laplacei[\frac{Dk^{-1}}{s}] - \laplacei[\frac{Dk^{-1}}{s+k}] - \laplacei[De^{-s}\frac{Dk^{-1}}{s}] - \laplacei[De^{-s}\frac{Dk^{-1}}{s+k}]\\
	x(t) &= \frac{D}{k}\laplacei[\frac{1}{s}] - \frac{D}{k}\laplacei[\frac{1}{s+k}] - \frac{D^{2}}{k}\laplacei[\frac{e^{-s}}{s}] - \frac{D^{2}}{k}\laplacei[\frac{e^{-s}}{s+k}]\\
	x(t) &= \frac{D}{k}(1) - \frac{D}{k}(e^{-kt}) - \frac{D^{2}}{k}(1\unitstep(t-1)) - \frac{D^{2}}{k}\left( e^{-kt}\unitstep(t-1) \right)\\
	x(t) &= \frac{D}{k}\left(1 - e^{-kt} - D\unitstep(t-1) - De^{-kt}\unitstep(t-1) \right)\\
\end{aligned}
\end{equation*}

\end{document}