%! Author = Len Washington III
%! Date = 9/11/24

% Preamble
\documentclass[
	date={September 11{,} 2024}
]{math486notes}

% Document
\begin{document}

\[ AUC = \int_{t_{1}}^{t_{2}} c(t)dt,\ \ [AUC] = \frac{MT}{Volume}  \]

\begin{equation*}
\begin{aligned}
	\bar{c(t)} &= \frac{1}{t_{2} - t_{1}}\int_{t_{1}}^{t_{2}}
\end{aligned}
\end{equation*}

\section{Half-life}\label{sec:half-life}
The time to reduce by $\frac{1}{2}$,
\begin{example}{Find $\tau_{\frac{1}{2}}$}
	\begin{equation*}
	\begin{aligned}
		\frac{D}{2} &= De^{-k\tau_{\frac{1}{2}}}\\
		\frac{1}{2} &= e^{-k\tau_{\frac{1}{2}}}\\
		\ln\left( \frac{1}{2} \right) &= -k\tau_{\frac{1}{2}}\\
		k &= \frac{\ln\left( \frac{1}{2} \right)}{\tau_{\frac{1}{2}}}\\
	\end{aligned}
	\end{equation*}
\end{example}

\begin{example}
	One compartment (plasma) with inhection
	\[ \frac{dx}{dt} = -kx,\ \ k > 0,\ \ x(0) = D \]
	Solution:
	\[ x(t) = De^{-kt} \]
	This is exponential decay
	\begin{equation}
		c(t) = \frac{x(t)}{V_{D}} = \frac{D}{V_{D}}e^{-kt}
		\label{eq:auc-for-example}
	\end{equation}
	\begin{equation*}
	\begin{aligned}
		AUC = \int_{0}^{\infty} x(t)dt = \frac{D}{k}
	\end{aligned}
	\end{equation*}
	Total amount eliminated = $kAUC = D$
\end{example}

\begin{example}{Patient}
	A patient gets a \emph{loading} does of 400mg of a drug.
	\begin{equation*}
	\begin{aligned}
		V_{D} &= 30L\\
		k &= 0.115 hr^{-1} (\mbox{removal rate})\\
		\halflife &= \frac{\ln 2}{}
	\end{aligned}
	\end{equation*}
	Assume a simple one compartment model as above with injection $D=400$ mg at $t=0$. What is the concentration after 4 hours.
	\begin{equation*}
	\begin{aligned}
		c(t) &= \frac{400}{30}e^{-0.115(4)}\\
			 &= 8.4 \mbox{mg}/\mbox{L}
	\end{aligned}
	\end{equation*}
\end{example}

\section{Alternate formulation}\label{sec:alternate-formulation}
One compartment model injection at $t=0$.
\begin{equation}
	\frac{dx}{dt} = -kx + D\delta(t),\ \ x(0) = 0
	\label{eq:create-name}
\end{equation}

\subsection{Properties}\label{subsec:properties}
\begin{equation}
	\int_{-\infty}^{\infty} \delta(t) dt = 1
	\label{eq:delta-dirac-1}
\end{equation}

\begin{equation}
	\int_{-\infty}^{\infty} \delta(t)f(t) dt = f(0)
	\label{eq:delta-dirac-2}
\end{equation}

\subsection{Dimensional Analysis}\label{subsec:dimensional-analysis}
\begin{equation*}
\begin{aligned}
	\frac{dx}{dt} &= -kx + D\delta(t)\\
	\left[ \frac{dx}{dt} \right] &= \frac{M}{T}\\
	&= [kx]\\
	[k] &= \frac{1}{T}\\
	[D\delta(t)] &= \frac{M}{T}\\
	[\delta(t)] &= \frac{1}{T}\\
\end{aligned}
\end{equation*}
Check: Since $\int_{-\infty}^{\infty} \delta(t)dt = 1$

\section{Method of Solution to Integral Transforms}\label{sec:method-of-solution-to-integral-transforms}
$\laplace[~]$ = Laplace Transform Operator

Solve~\eqref{eq:create-name} using Laplace Transforms:
\begin{equation*}
\begin{aligned}
	X(s) &= \laplace[x(t)]\\
		 &= \int_{0}^{\infty} e^{-st} x(t)dt
\end{aligned}
\end{equation*}
Rules:
$\dots$

\begin{equation*}
\begin{aligned}
	\laplace[\frac{dx}{dt}] &= \laplace[ -kx + D\delta(t) ]\\
							&= \laplace[-kx] + \laplace[D\delta(t)]\\
							&= -k\laplace[x(t)] + D\laplace[\delta(t)]\\
	sX(s) - x(0) &= -kX(s) + D\times1\\
	sX(s) - 0 &= -kX(s) + D\\
	sX(s) + kX(s) &= D\\
	(s+k)X(s) &= D\\
	X(s) &= \frac{D}{s+k}\\
	\laplacei[X(s)] &= D\laplacei[\frac{1}{s+k}]\\
	x(t) &= De^{-k}\\
\end{aligned}
\end{equation*}

\section{Multiple Dosing}\label{sec:multiple-dosing}
Two injections
Injection at $t=0$ and a 2nd injection at $t=t_{1}$.
\[ D\delta(t) + D\delta(t - t_{1}) \]
\begin{equation}
	\frac{dx}{dt} = -kx + D\delta(t) + D\delta(t - t_{1}),\ \ x(0) = 0
	\label{eq:two-injections}
\end{equation}

Apply Laplace Transforms to~\eqref{eq:two-injections}.

\begin{equation*}
\begin{aligned}
	X(s) &= \laplace[x(t)]\\
	\laplace[\delta(t)] &= 1\\
	\laplace[ \delta(t - t_{1}) ] &= \int_{0}^{\infty} \dots\\
		&= e^{-st_{1}}
\end{aligned}
\end{equation*}
\begin{equation*}
\begin{aligned}
	\laplace[\frac{dx}{dt}] &= \laplace{-kx} + D\laplace[\delta(t)] + D\laplace[\delta(t-t_{1})]\\
	sX(s) - x(0) &= -kX(s) + D(1) + De^{-st_{1}}\\
	sX(s) - 0 + kX(s) &= D + De^{-st_{1}}\\
	(s+k)X(s) &= D + De^{-st_{1}}\\
	X(s) &= \frac{D}{s+k} + \frac{De^{-st_{1}}}{s+k}\\
\end{aligned}
\end{equation*}

\end{document}